Use new binder_inductive in LC and ILC

thys/Infinitary_Lambda_Calculus/ILC_Beta.thy
@@ -8,41 +8,35 @@ begin
 
 (* *)
 
-type_synonym T = "itrm \<times> itrm"
+abbreviation Tsupp :: "itrm \<Rightarrow> itrm \<Rightarrow> ivar set" where 
+"Tsupp e1 e2 \<equiv> FFVars e1 \<union> FFVars e2"
 
-definition Tperm :: "(ivar \<Rightarrow> ivar) \<Rightarrow> T \<Rightarrow> T" where 
-"Tperm f \<equiv> map_prod (irrename f) (irrename f)"
-
-fun Tsupp :: "T \<Rightarrow> ivar set" where 
-"Tsupp (e1,e2) = FFVars e1 \<union> FFVars e2"
-
-lemma small_Tsupp: "small (Tsupp t)"
+lemma small_Tsupp: "small (Tsupp t1 t2)"
   unfolding small_def
-  by (cases t) (auto intro!: var_iterm_pre_class.Un_bound iterm.card_of_FFVars_bounds)
+  by (auto intro!: var_iterm_pre_class.Un_bound iterm.card_of_FFVars_bounds)
 
-lemma Tvars_dsset: "(Tsupp t - dsset xs) \<inter> dsset xs = {}" "|Tsupp t - dsset xs| <o |UNIV::ivar set|"
+lemma Tvars_dsset: "(Tsupp t1 t2 - dsset xs) \<inter> dsset xs = {}" "|Tsupp t1 t2 - dsset xs| <o |UNIV::ivar set|"
 apply auto by (meson card_of_minus_bound small_Tsupp small_def)
 
-binder_inductive istep :: "itrm \<Rightarrow> itrm \<Rightarrow> bool" where
-  Beta: "istep (iApp (iLam xs e1) es2) (itvsubst (imkSubst xs es2) e1)" binds "dsset xs"
+inductive istep :: "itrm \<Rightarrow> itrm \<Rightarrow> bool" where
+  Beta: "istep (iApp (iLam xs e1) es2) (itvsubst (imkSubst xs es2) e1)"
 | iAppL: "istep e1 e1' \<Longrightarrow> istep (iApp e1 es2) (iApp e1' es2)"
 | iAppR: "istep (snth es2 i) e2' \<Longrightarrow> istep (iApp e1 es2) (iApp e1 (supd es2 i e2'))"
-| Xi: "istep e e' \<Longrightarrow> istep (iLam xs e) (iLam xs e')" binds "dsset xs"
-where perm: Tperm supp: Tsupp
-  unfolding isPerm_def Tperm_def  
+| Xi: "istep e e' \<Longrightarrow> istep (iLam xs e) (iLam xs e')"
+
+binder_inductive istep where
+  Beta binds "dsset xs"
+| Xi binds "dsset xs"
+for perms: irrename irrename and supps: FFVars FFVars
+  unfolding isPerm_def  
   using small_Un small_def iterm.card_of_FFVars_bounds
-         apply (auto simp: iterm.rrename_id0s map_prod.comp iterm.rrename_comp0s infinite_UNIV) [5]
-  using var_sum_class.Un_bound unfolding small_def apply blast
-  subgoal by fastforce
-  subgoal for \<sigma> R B t
-    unfolding split_beta
-    apply(elim disjE)
-    subgoal apply(rule disjI4_1)
-      subgoal apply(elim exE) subgoal for xs e1 es2
+         apply (auto simp: iterm.rrename_id0s map_prod.comp iterm.rrename_comps infinite_UNIV) [12]
+  subgoal for R B \<sigma> x1 x2
+    apply (elim disj_forward exE conjE)
+    subgoal for xs e1 es2
         apply(rule exI[of _ "dsmap \<sigma> xs"])
         apply(rule exI[of _ "irrename \<sigma> e1"])  
         apply(rule exI[of _ "smap (irrename \<sigma>) es2"])  
-        apply(cases t) unfolding isPerm_def small_def Tperm_def 
         apply (simp add: iterm.rrename_comps) apply(subst irrename_itvsubst_comp) apply auto
         apply(subst imkSubst_smap_irrename_inv) unfolding isPerm_def apply auto 
         apply(subst irrename_eq_itvsubst_iVar'[of _ e1]) unfolding isPerm_def apply auto
@@ -54,45 +48,37 @@ where perm: Tperm supp: Tsupp
           subgoal using card_SSupp_itvsubst_imkSubst_irrename_inv isPerm_def by auto
           subgoal for x apply simp apply(subst iterm.subst(1))
             subgoal using card_SSupp_imkSubst_irrename_inv[unfolded isPerm_def] by auto
-            subgoal by simp . . . . . 
+            subgoal by simp . . .
       (* *)
-  subgoal apply(rule disjI4_2)
-    subgoal apply(elim exE) subgoal for e1 e1' es2 
+  subgoal for e1 e1' es2 
       apply(rule exI[of _ "irrename \<sigma> e1"]) apply(rule exI[of _ "irrename \<sigma> e1'"]) 
       apply(rule exI[of _ "smap (irrename \<sigma>) es2"]) 
-      apply(cases t) unfolding isPerm_def small_def Tperm_def 
-      by (simp add: iterm.rrename_comps) . . 
+      by (simp add: iterm.rrename_comps)
     (* *)
-  subgoal apply(rule disjI4_3)
-    subgoal apply(elim exE) subgoal for es2 i e2' e1 
+  subgoal for es2 i e2' e1 
       apply(rule exI[of _ "smap (irrename \<sigma>) es2"]) 
       apply(rule exI[of _ i])
       apply(rule exI[of _ "irrename \<sigma> e2'"]) 
-      apply(rule exI[of _ "irrename \<sigma> e1"])
-      apply(cases t) unfolding isPerm_def small_def Tperm_def 
-      apply (simp add: iterm.rrename_comps) . . .
+      apply(rule exI[of _ "irrename \<sigma> e1"]) 
+      apply (simp add: iterm.rrename_comps) .
     (* *)
-  subgoal apply(rule disjI4_4)
-    subgoal apply(elim exE) subgoal for e e' xs
+  subgoal for e e' xs
       apply(rule exI[of _ "irrename \<sigma> e"]) apply(rule exI[of _ "irrename \<sigma> e'"]) 
-      apply(rule exI[of _ "dsmap \<sigma> xs"])
-      apply(cases t) unfolding isPerm_def small_def Tperm_def  
-      by (simp add: iterm.rrename_comps) . . . 
-  subgoal premises prems for R B t
-    using prems(2-)
-    unfolding Tperm_def split_beta apply safe
+      apply(rule exI[of _ "dsmap \<sigma> xs"]) 
+      by (simp add: iterm.rrename_comps) .
+  subgoal premises prems for R B x1 x2
+    using prems(2-) apply safe
     subgoal for xs e1 es2  
-      using refresh[OF Tvars_dsset, of xs t]  apply safe
+      using refresh[OF Tvars_dsset, of xs x1 x2]  apply safe
       subgoal for f
         apply(rule exI[of _ "f ` (dsset xs)"])  
         apply(intro conjI)
-        subgoal by (metis dsset_card_ls dstream.set_map)
-        subgoal unfolding id_on_def by auto (metis DiffI Int_emptyD image_eqI)
+        subgoal by (simp add: Diff_Int_distrib)
         subgoal apply(rule disjI4_1)
           apply(rule exI[of _ "dsmap f xs"]) 
           apply(rule exI[of _ "irrename f e1"]) 
           apply(rule exI[of _ "es2"]) 
-          apply(cases t)  apply simp apply(intro conjI)
+          apply simp apply(intro conjI)
           subgoal apply(subst iLam_irrename[of "f"]) unfolding id_on_def by auto
           subgoal apply(subst irrename_eq_itvsubst_iVar)
             subgoal unfolding isPerm_def by auto
@@ -111,96 +97,32 @@ where perm: Tperm supp: Tsupp
                 apply(rule exI[of _ "{}"])  
                 apply(intro conjI)
                 subgoal by simp
-                subgoal unfolding isPerm_def small_def by auto 
-                subgoal apply(rule disjI4_2) 
-                  apply(rule exI[of _ "e1"]) 
-                  apply(rule exI[of _ "e1'"])
-                  apply(rule exI[of _ "es2"]) 
-                  apply(cases t) apply simp . .
+                subgoal by auto .
                   (* *)
               subgoal for e1 e2 es2' 
                 apply(rule exI[of _ "{}"])  
                 apply(intro conjI)
                 subgoal by simp
-                subgoal unfolding isPerm_def small_def by auto 
-                subgoal apply(rule disjI4_3) 
-                  apply(rule exI[of _ "e1"]) 
-                  apply(rule exI[of _ "e2"])
-                  apply(rule exI[of _ "es2'"]) 
-                  apply(cases t) apply auto . .
+                subgoal unfolding isPerm_def small_def by auto .
                   (* *) 
               subgoal for e e' xs
-                using refresh[OF Tvars_dsset, of xs t]  apply safe
+                using refresh[OF Tvars_dsset, of xs x1 x2]  apply safe
                 subgoal for f
                   apply(rule exI[of _ "f ` (dsset xs)"])  
                   apply(intro conjI)
-                  subgoal by (metis dsset_card_ls dstream.set_map)
-                  subgoal unfolding id_on_def by auto (metis DiffI Int_emptyD image_eqI)
+                  subgoal by (metis Diff_Int_distrib Diff_empty dstream.set_map)
                   subgoal apply(rule disjI4_4)  
                     apply(rule exI[of _ "irrename f e"]) 
                     apply(rule exI[of _ "irrename f e'"]) 
                     apply(rule exI[of _ "dsmap f xs"])
-                    apply(cases t)  apply simp apply(intro conjI)
+                    apply simp apply(intro conjI)
                     subgoal apply(subst iLam_irrename[of "f"]) unfolding id_on_def by auto
                     subgoal apply(subst iLam_irrename[of "f"]) unfolding id_on_def by auto
                     . . . .
                   done
 
-corollary strong_induct_istep[consumes 2, case_names Beta iAppL iAppR Xi]: 
-assumes par: "\<And>p. small (Psupp p)"
-and st: "istep t1 t2"  
-and Beta: "\<And>xs e1 es2 p. 
-  dsset xs \<inter> Psupp p = {} \<Longrightarrow> dsset xs \<inter> \<Union>(FFVars`(sset es2)) = {} \<Longrightarrow> 
-  R p (iApp (iLam xs e1) es2) (itvsubst (imkSubst xs es2) e1)"
-and iAppL: "\<And>e1 e1' es2 p. 
-  istep e1 e1' \<Longrightarrow> (\<forall>p'. R p' e1 e1') \<Longrightarrow> 
-  R p (iApp e1 es2) (iApp e1' es2)"
-and iAppR: "\<And>e1 es2 i e2' p. 
-  istep (snth es2 i) e2' \<Longrightarrow> (\<forall>p'. R p' (es2 !! i) e2') \<Longrightarrow> 
-  R p (iApp e1 es2) (iApp e1 (supd es2 i e2'))"
-and Xi: "\<And>e e' xs p. 
-  dsset xs \<inter> Psupp p = {} \<Longrightarrow> 
-  istep e e' \<Longrightarrow> (\<forall>p'. R p' e e') \<Longrightarrow> 
-  R p (iLam xs e) (iLam xs e')" 
-shows "R p t1 t2"
-unfolding istep.alt_def
-apply(subgoal_tac "case (t1,t2) of (t1, t2) \<Rightarrow> R p t1 t2")
-  subgoal by simp
-  subgoal using par st apply(elim istep.strong_induct[where R = "\<lambda>p (t1,t2). R p t1 t2"])
-    subgoal unfolding istep.alt_def by simp
-    subgoal for p B t
-    unfolding istep.alt_def[symmetric] apply(elim disjE exE case_prodE)
-      subgoal for _ _ xs e1 es2 using Beta[of xs p es2 e1] by force
-      subgoal using iAppL by auto  
-      subgoal using iAppR by auto  
-      subgoal using Xi by auto . . .
-
-corollary strong_induct_istep''[consumes 1, case_names Bound Beta iAppL iAppR Xi]: 
-assumes st: "istep t1 t2"
-and par: "\<And>p. |Psupp p| <o |UNIV::ivar set|"
-and Beta: "\<And>xs e1 es2 p. 
-  dsset xs \<inter> Psupp p = {} \<Longrightarrow> dsset xs \<inter> \<Union>(FFVars`(sset es2)) = {} \<Longrightarrow> 
-  R (iApp (iLam xs e1) es2) (itvsubst (imkSubst xs es2) e1) p"
-and iAppL: "\<And>e1 e1' es2 p. 
-  istep e1 e1' \<Longrightarrow> (\<forall>p'. R e1 e1' p') \<Longrightarrow> 
-  R (iApp e1 es2) (iApp e1' es2) p"
-and iAppR: "\<And>e1 es2 i e2' p. 
-  istep (snth es2 i) e2' \<Longrightarrow> (\<forall>p'. R (es2 !! i) e2' p') \<Longrightarrow> 
-  R (iApp e1 es2) (iApp e1 (supd es2 i e2')) p"
-and Xi: "\<And>e e' xs p. 
-  dsset xs \<inter> Psupp p = {} \<Longrightarrow> 
-  istep e e' \<Longrightarrow> (\<forall>p'. R e e' p') \<Longrightarrow> 
-  R (iLam xs e) (iLam xs e') p" 
-shows "\<forall>p. (R t1 t2 p)"
-using strong_induct_istep[of Psupp t1 t2 "\<lambda>p t1 t2. R t1 t2 p"] assms unfolding small_def by auto
-
-(* Also inferring equivariance from the general infrastructure: *)
-corollary irrename_istep:
-assumes f: "bij f" "|supp f| <o |UNIV::ivar set|" 
-and r: "istep e e'" 
-shows "istep (irrename f e) (irrename f e')"
-using assms unfolding istep.alt_def using istep.equiv[of "(e,e')" f]
-unfolding Tperm_def isPerm_def by auto
+thm istep.strong_induct
+thm istep.equiv
 
 (* Other properties: *)
 
