thys/Untyped_Lambda_Calculus/LC_Beta.thy
@@ -8,63 +8,39 @@ begin
 
 (* *)
 
-fun Tperm where "Tperm f (a,b) = ((rrename f a,rrename f b))"
-fun Tsupp where "Tsupp (a,b) = FFVars a \<union> FFVars b"
-lemma fresh: "\<exists>xx. xx \<notin> Tsupp (t :: trm \<times> trm)"
-  using Tsupp.simps[of "fst t" "snd t"] unfolding prod.collapse
+abbreviation Tsupp where "Tsupp a b \<equiv> FFVars a \<union> FFVars b"
+lemma fresh: "\<exists>xx. xx \<notin> Tsupp (t1::trm) t2"
+  unfolding prod.collapse
   by (metis (no_types, lifting) exists_var finite_iff_le_card_var term.Un_bound term.set_bd_UNIV)
 
-binder_inductive step :: "trm \<Rightarrow> trm \<Rightarrow> bool" where
-  Beta: "step (App (Lam x e1) e2) (tvsubst (Var(x:=e2)) e1)" binds "{x}"
+inductive step :: "trm \<Rightarrow> trm \<Rightarrow> bool" where
+  Beta: "step (App (Lam x e1) e2) (tvsubst (Var(x:=e2)) e1)"
 | AppL: "step e1 e1' \<Longrightarrow> step (App e1 e2) (App e1' e2)"
 | AppR: "step e2 e2' \<Longrightarrow> step (App e1 e2) (App e1 e2')"
-| Xi: "step e e' \<Longrightarrow> step (Lam x e) (Lam x e')" binds "{x}"
-where perm: Tperm supp: Tsupp
-   \<comment> \<open>properties of LS-Nominal sets and monotonicity\<close>
+| Xi: "step e e' \<Longrightarrow> step (Lam x e) (Lam x e')"
+
+binder_inductive step where
+  Beta binds x
+| Xi binds x
+for perms: rrename rrename and supps: FFVars FFVars
+   \<comment> \<open>properties of LS-Nominal sets\<close>
   apply (auto simp: o_def split_beta term.rrename_comps fun_eq_iff isPerm_def
-    small_def term.card_of_FFVars_bounds term.Un_bound) [6]
+    small_def term.card_of_FFVars_bounds term.Un_bound infinite_UNIV) [12]
   subgoal for \<sigma> R B t  \<comment> \<open>equivariance\<close>
     by (elim disj_forward case_prodE)
       (auto simp: isPerm_def term.rrename_comps rrename_tvsubst_comp
          | ((rule exI[of _ "\<sigma> _"] exI)+, (rule conjI)?, rule refl)
          | ((rule exI[of _ "\<sigma> _"])+; auto))+
-  subgoal premises prems for R B t  \<comment> \<open>refreshability\<close>
-    using fresh[of t] prems(2-) unfolding isPerm_def conj_assoc[symmetric] split_beta
+  subgoal premises prems for R B x1 x2  \<comment> \<open>refreshability\<close>
+    using fresh[of x1 x2] prems(2-) unfolding isPerm_def conj_assoc[symmetric] split_beta
     unfolding ex_push_inwards conj_disj_distribL ex_disj_distrib
-    by (elim disj_forward exE; simp)
-      ((rule exI, rule conjI[rotated], assumption) |
-        (((rule exI conjI)+)?, rule Lam_refresh tvsubst_refresh) |
-        (cases t; auto))+
+    apply (elim disj_forward exE; simp)
+     apply (metis Lam_eq_tvsubst Lam_inject_swap singletonD)
+    by blast
   done
 
-corollary strong_induct_step[consumes 2, case_names Beta AppL AppR Xi]: 
-assumes par: "\<And>p. small (Psupp p)" and st: "step t1 t2"  
-and Beta: "\<And>x e1 e2 p. x \<notin> Psupp p \<Longrightarrow> x \<notin> FFVars_term e2 \<Longrightarrow> R p (App (Lam x e1) e2) (tvsubst (VVr(x := e2)) e1)"
-and AppL: "\<And>e1 e1' e2 p. step e1 e1' \<Longrightarrow> (\<forall>p'. R p' e1 e1') \<Longrightarrow> R p (App e1 e2) (App e1' e2)"
-and AppR: "\<And>e1 e2 e2' p. step e2 e2' \<Longrightarrow> (\<forall>p'. R p' e2 e2') \<Longrightarrow> R p (App e1 e2) (App e1 e2')"
-and Xi: "\<And>e e' x p. x \<notin> Psupp p \<Longrightarrow> step e e' \<Longrightarrow> (\<forall>p'. R p' e e') \<Longrightarrow> R p (Lam x e) (Lam x e')" 
-shows "R p t1 t2"
-unfolding step.alt_def apply(subgoal_tac "case (t1,t2) of (t1, t2) \<Rightarrow> R p t1 t2")
-  subgoal by simp
-  subgoal using par st apply(elim step.strong_induct[where R = "\<lambda>p (t1,t2). R p t1 t2"])
-    subgoal unfolding step.alt_def by simp
-    subgoal for p B t
-    unfolding step.alt_def[symmetric] apply(elim disjE exE case_prodE)
-      subgoal for _ _ x e1 e2  using Beta[of x p e2 e1] by auto
-      subgoal using AppL by auto  
-      subgoal using AppR by auto  
-      subgoal using Xi by auto . . .
-
-corollary rrename_step:
-assumes f: "bij f" "|supp f| <o |UNIV::var set|" and r: "step e e'" 
-shows "step (rrename f e) (rrename f e')"
-using assms unfolding step.alt_def using step.equiv[of "(e,e')" f] unfolding isPerm_def by auto
-
-(* Output of binder_inductive
-thm step.alt_def
 thm step.strong_induct
 thm step.equiv
-*)
 
 (* ALTERNATIVE manual instantiation without the automation provided by binder_inductive *)
 (*
@@ -258,25 +234,6 @@ subgoal for R tt1 tt2 apply(rule iffI)
     \<^cancel>\<open>Xi: \<close>
     subgoal apply(rule disjI4_4) by auto . . .
 *)
-
-corollary strong_induct_step'[consumes 1, case_names Bound Beta AppL AppR Xi]: 
-assumes st: "step t1 t2"
-and par: "\<And>p. |Psupp p| <o |UNIV::var set|"
-and Beta: "\<And>x e1 e2 p. 
-  x \<notin> Psupp p \<Longrightarrow> x \<notin> FFVars_term e2 \<Longrightarrow> 
-  R (App (Lam x e1) e2) (tvsubst (VVr(x := e2)) e1) p"
-and AppL: "\<And>e1 e1' e2 p. 
-  step e1 e1' \<Longrightarrow> (\<forall>p'. R e1 e1' p') \<Longrightarrow> 
-  R (App e1 e2) (App e1' e2) p"
-and AppR: "\<And>e1 e2 e2' p. 
-  step e2 e2' \<Longrightarrow> (\<forall>p'. R e2 e2' p') \<Longrightarrow> 
-  R (App e1 e2) (App e1 e2') p"
-and Xi: "\<And>e e' x p. 
-  x \<notin> Psupp p \<Longrightarrow> 
-  step e e' \<Longrightarrow> (\<forall>p'. R e e' p') \<Longrightarrow> 
-  R (Lam x e) (Lam x e') p" 
-shows "\<forall>p. R t1 t2 p"
-using strong_induct_step[of Psupp t1 t2 "\<lambda>p t1 t2. R t1 t2 p"] assms unfolding small_def by auto
 
 (* Other properties: *)
 
